Foundation/Modal/Kripke/AxiomPoint3.lean
@@ -11,6 +11,9 @@ namespace Frame
 
 class IsPiecewiseStronglyConnected (F : Frame) extends _root_.IsPiecewiseStronglyConnected F.Rel
 
+lemma ps_connected [F.IsPiecewiseStronglyConnected] : ∀ {x y z : F.World}, x ≺ y → x ≺ z →  y ≺ z ∨ z ≺ y := by
+  apply IsPiecewiseStronglyConnected.ps_connected
+
 end Frame
 
 
