Foundation/Modal/Kripke/Filtration.lean
@@ -1,5 +1,8 @@
 import Mathlib.Data.Set.Finite.Powerset
 import Foundation.Modal.Kripke.Closure
+import Foundation.Modal.Kripke.Rooted
+import Foundation.Modal.Kripke.AxiomPoint3
+import Foundation.Modal.Kripke.AxiomWeakPoint3
 
 universe u v
 
@@ -222,7 +225,7 @@ abbrev finestFiltrationTransitiveClosureModel (M : Model) (T : FormulaSet ℕ) [
 namespace finestFiltrationTransitiveClosureModel
 
 open Relation in
-instance filterOf [trans : IsTrans _ M.Rel] : FilterOf (finestFiltrationTransitiveClosureModel M T) M T where
+instance filterOf [trans : M.IsTransitive] : FilterOf (finestFiltrationTransitiveClosureModel M T) M T where
   def_rel_forth := by
     intro x y hxy;
     apply Relation.TransGen.single;
@@ -247,17 +250,80 @@ instance filterOf [trans : IsTrans _ M.Rel] : FilterOf (finestFiltrationTransiti
       apply FilterEqvQuotient.iff_of_eq euv (by assumption) |>.mpr;
       intro z Rvz;
       apply FilterEqvQuotient.iff_of_eq exw (by assumption) |>.mp hx;
-      exact _root_.trans Rwv Rvz;
+      exact M.trans Rwv Rvz;
 
 lemma isFinite (T_finite : T.Finite) : (finestFiltrationTransitiveClosureModel M T).IsFinite where
   world_finite := FilterEqvQuotient.finite T_finite
 
-instance isReflexive [M.IsPreorder] : (finestFiltrationTransitiveClosureModel M T).IsReflexive := finestFiltrationTransitiveClosureModel.filterOf.isReflexive
 instance isTransitive : (finestFiltrationTransitiveClosureModel M T).IsTransitive where
-instance isSerial [M.IsTransitive] [M.IsSerial] : (finestFiltrationTransitiveClosureModel M T).IsSerial := finestFiltrationTransitiveClosureModel.filterOf.isSerial
-instance isSymmetric [M.IsSymmetric] : (finestFiltrationTransitiveClosureModel M T).IsSymmetric := Frame.TransGen.isSymmetric
-instance isPreorder [M.IsPreorder] : (finestFiltrationTransitiveClosureModel M T).IsPreorder where
-instance isEquiv [M.IsEquivalence] : (finestFiltrationTransitiveClosureModel M T).IsEquivalence where
+instance isSerial [trans : M.IsTransitive] [serial : M.IsSerial] : (finestFiltrationTransitiveClosureModel M T).IsSerial := finestFiltrationTransitiveClosureModel.filterOf.isSerial
+instance isSymmetric [symm : M.IsSymmetric] : (finestFiltrationTransitiveClosureModel M T).IsSymmetric := Frame.TransGen.isSymmetric
+instance isReflexive [preorder : M.IsPreorder] : (finestFiltrationTransitiveClosureModel M T).IsReflexive := finestFiltrationTransitiveClosureModel.filterOf.isReflexive
+instance isPreorder [preorder : M.IsPreorder] : (finestFiltrationTransitiveClosureModel M T).IsPreorder where
+instance isEquiv [equiv : M.IsEquivalence] : (finestFiltrationTransitiveClosureModel M T).IsEquivalence where
+
+instance rooted_isPiecewiseStronglyConvergent [preorder : M.IsPreorder] [ps_convergent : M.IsPiecewiseStronglyConvergent] : (finestFiltrationTransitiveClosureModel (M↾r) T).IsPiecewiseStronglyConvergent where
+  ps_convergent := by
+    rintro X ⟨y, (rfl | Rry)⟩ ⟨z, (rfl | Rrz)⟩ RXY RXZ;
+    . simp only [and_self];
+      use ⟦⟨z, by tauto⟩⟧;
+      apply Relation.TransGen.single;
+      suffices z ≺ z by tauto;
+      apply M.refl;
+    . use ⟦⟨z, by tauto⟩⟧;
+      constructor;
+      . apply Relation.TransGen.single;
+        suffices y ≺ z by tauto;
+        exact HRel.TransGen.unwrap Rrz;
+      . apply Relation.TransGen.single;
+        suffices z ≺ z by tauto;
+        apply IsRefl.refl ;
+    . use ⟦⟨y, by tauto⟩⟧;
+      constructor;
+      . apply Relation.TransGen.single;
+        suffices y ≺ y by tauto;
+        apply IsRefl.refl;
+      . apply Relation.TransGen.single;
+        suffices z ≺ y by tauto;
+        exact HRel.TransGen.unwrap Rry;
+    . replace Rry := HRel.TransGen.unwrap Rry;
+      replace Rrz := HRel.TransGen.unwrap Rrz;
+      obtain ⟨u, Ruy, Ruz⟩ := M.ps_convergent Rry Rrz;
+      use ⟦⟨u, by
+        right;
+        apply Relation.TransGen.single;
+        exact IsTrans.trans _ _ _ Rry Ruy;
+      ⟩⟧;
+      constructor;
+      . exact Relation.TransGen.single $ by tauto;
+      . exact Relation.TransGen.single $ by tauto;
+
+instance rooted_isPiecewiseStronglyConnected [preorder : M.IsPreorder] [ps_connected : M.IsPiecewiseStronglyConnected] : (finestFiltrationTransitiveClosureModel (M↾r) T).IsPiecewiseStronglyConnected where
+  ps_connected := by
+    rintro X ⟨y, (rfl | Rry)⟩ ⟨z, (rfl | Rrz)⟩ RXY RXZ;
+    . simp only [or_self];
+      apply Relation.TransGen.single;
+      suffices z ≺ z by tauto;
+      apply IsRefl.refl;
+    . left;
+      apply Relation.TransGen.single;
+      suffices y ≺ z by tauto;
+      exact Rrz.unwrap;
+    . right;
+      apply Relation.TransGen.single;
+      suffices z ≺ y by tauto;
+      exact Rry.unwrap;
+    . replace Rry := Rry.unwrap;
+      replace Rrz := Rrz.unwrap;
+      rcases M.ps_connected Rry Rrz with (Ryz | Rrw);
+      . left;
+        apply Relation.TransGen.single;
+        tauto;
+      . right;
+        apply Relation.TransGen.single;
+        tauto;
+
+
 
 end finestFiltrationTransitiveClosureModel
 
